\documentclass[a5paper]{article}
\usepackage{amsmath}
\usepackage{amssymb}
\usepackage[top=1cm,right=1cm,bottom=2cm,left=1cm]{geometry}
\setlength\parindent{0pt}
\setlength\parskip{1em}
\begin{document}
\newcommand   \C            {\mathbf{C}}
\newcommand   \R            {\mathbf{R}}
\renewcommand \L            {\mathcal{L}}
\newcommand   \F            {\mathbf{F}}
\renewcommand \P            {\mathcal{P}}
\newcommand   \M            {\mathcal{M}}
\newcommand   \E            {\mathcal{E}}
\newcommand   \op           {\operatorname}
\newcommand   \A            {\mathcal{A}}
\newcommand   \Q            {\mathcal{Q}}
\newcommand   \conj[1]      {\overline{#1}}

    4.2.
    Prove that if $w,z \in \C$, then $\big| |w| - |z| \big| \le |w - z|$.
\begin{align*}
        |w - z|^2   &= (w - z) (\conj{w - z}) \\
                    &= (w - z) (\conj{w} - \conj{z}) \\
                    &= w\conj{w} - w\conj{z} - z\conj{w} + z\conj{z} \\
                    &= |w|^2 - w\conj{z} - \conj{w}z + |z|^2 \\
                    &= |w|^2 - w\conj{z} - \conj{w}\ \conj{\conj{z}} + |z|^2  \\
                    &= |w|^2 - w\conj{z} - \conj{w \conj{z}}         + |z|^2  \\
                    &= |w|^2 - 2 \op{Im}(w\conj{z})i                 + |z|^2  \\
                    &\ge |w|^2 - 2 |w\conj{z}|   + |z|^2  \\
                    &= |w|^2 - 2 |w| |\conj{z}|  + |z|^2  \\
                    &= |w|^2 - 2 |w| |z| + |z|^2 \\
                    &= (|w| - |z|)^2 \\
                    &= \big| |w| - |z| \big|^2 .
\end{align*}
    Taking the square roots of both sides now gives the desired inequality.

    Geometric interpretation: the length of one side of a triangle is greater than or equal to the difference in the lengths of the other two sides.
\end{document}
