\documentclass[a5paper]{article}
\usepackage{amsmath}
\usepackage{amssymb}
\usepackage[top=1cm,right=1cm,bottom=2cm,left=1cm]{geometry}
\setlength\parindent{0pt}
\setlength\parskip{1em}
%
\begin{document}
\newcommand   \C           {\mathbf{C}}
\newcommand   \R           {\mathbf{R}}
\renewcommand \L           {\mathcal{L}}
\newcommand   \F           {\mathbf{F}}
\renewcommand \P           {\mathcal{P}}
\newcommand   \M           {\mathcal{M}}
\newcommand   \E           {\mathcal{E}}
\newcommand   \op          {\operatorname}

    3.D.12.
    Suppose $V$ is finite-dimensional and $S,T,U \in \L(V)$ and $STU = I$.
    Show that $T$ is invertible and that $T^{-1} = US$.
    \hfill

    First, $I = STU = (ST)U$.

    Because $ST$ and $U$ are both operators on a finite-dimensional vector space, we can use the multiplicative commutativity shown in proof 3.68 to get $U(ST) = I$.

    Hence $I = U(ST) = (US)T$.

    Again using proof 3.68, this implies that $T(US) = I$.

    Thus $US$ and $T$ are invertible with $T^{-1} = US$.
\end{document}
