\documentclass[a5paper]{article}
\usepackage{amsmath}
\usepackage{amssymb}
\usepackage[top=1cm,right=1cm,bottom=2cm,left=1cm]{geometry}
\setlength\parindent{0pt}
\setlength\parskip{1em}
\begin{document}
\newcommand   \C           {\mathbf{C}}
\newcommand   \R           {\mathbf{R}}
\renewcommand \L           {\mathcal{L}}
\newcommand   \F           {\mathbf{F}}
\renewcommand \P           {\mathcal{P}}
\newcommand   \M           {\mathcal{M}}
\newcommand   \E           {\mathcal{E}}
\newcommand   \op          {\operatorname}
\newcommand   \A           {\mathcal{A}}
\newcommand   \Q           {\mathcal{Q}}

    3.D.22.
    Suppose $T \in \L(V)$ and $v_1,\dots,v_n$ is a basis of $V$.
    Prove that
\begin{align*}
        \M\big(T, (v_1,\dots,v_n) \big)\ \text{is invertible}\ \Longleftrightarrow\ T\ \text{is invertible}.
\end{align*}
    In both parts of the proof below, let $A = \M\big(T, (v_1,\dots,v_n) \big)$.

    First suppose $A$ is invertible.
    Then there exists an $n$-by-$n$ matrix $A^{-1}$ such that $AA^{-1}$ equals the identity matrix.

    Since $\M$ is an isomorphism, $\M$ is surjective onto $\F^{n,n}$.
    So there exists $S \in \L(V)$ such that $A^{-1} = \M\big( S, (v_1,\dots,v_n) \big)$.

    Suppose $v \in V$.
    Then
\begin{align*}
        \M(v) &= \M(Iv) \\
              &= \M(I)\M(v) \\
              &= A A^{-1} \M(v) \\
              &= \M(T) \M(S) \M(v) \\
              &= \M(T) \M(Sv) \\
              &= \M\big(T(Sv)\big) .
\end{align*}
    Since $\M$ is an isomorphism, $\M$ is injective.
    Hence the above equation implies that $v=T(Sv)$.
    Thus $v \in \op{range}T$.
    Hence $T$ is surjective.

    Thus $T$ is a surjective operator on a finite-dimensional vector space.
    Hence $T$ is invertible, completing the proof in one direction.

    Now suppose $T$ is invertible.
    In other words, there exists $T^{-1} \in \L(V)$ such that $TT^{-1}=T^{-1}T=I$.

    Let $B = \M\big(T^{-1}, (v_1,\dots,v_n) \big)$.
    Then we have
\begin{align*}
        AB = \M(T)\M(T^{-1}) = \M(T T^{-1}) = \M(I)
\end{align*}
    and
\begin{align*}
        BA = \M(T^{-1})\M(T) = \M(T^{-1} T) = \M(I) .
\end{align*}
    Hence $A$ is invertible, as desired.
\end{document}
