\documentclass[a5paper]{article}
\usepackage{amsmath}
\usepackage[top=1cm,right=1cm,bottom=1cm,left=1cm]{geometry}
\setlength\parindent{0pt}
\setlength\parskip{1em}
%
%\usepackage{xcolor}
%\pagecolor[rgb]{0.1,0.1,0.1}
%\color[rgb]{1.0,1.0,1.0}
%
\begin{document}
\newcommand   \C           {\mathbf{C}}
\newcommand   \R           {\mathbf{R}}
\renewcommand \L           {\mathcal{L}}
\newcommand   \F           {\mathbf{F}}
\renewcommand \P           {\mathcal{P}}
\newcommand   \M           {\mathcal{M}}
\newcommand   \question[1] {\textbf{\boldmath#1\unboldmath}\par}
\newcommand   \op          {\operatorname}

\question{
    3.C.3. Suppose $v_1,\dots,v_n$ is a basis of $V$ and $w_1,\dots,w_m$ is a basis of $W$.
}
\question{
    (a) Show that if $S,T \in \L(V,W)$, then $\M(S+T) = \M(S)+\M(T)$.
}

    Suppose $\M(S) = A$ and $\M(T) = B$.
    Then for $k = 1,\dots,n$,
\begin{align*}
        (S+T)v_k &= Sv_k + Tv_k \\
                 &= \sum_{j=1}^m A_{j,k}w_j + \sum_{j=1}^m B_{j,k}w_j \\
                 &= \sum_{j=1}^m (A_{j,k}w_j + B_{j,k}w_j) \\
                 &= \sum_{j=1}^m (A_{j,k} + B_{j,k}) w_j .
\end{align*}
    Thus $\M(S + T)$ is the $m$ by $n$ matrix in which each entry is the sum of the corresponding entries in $\M(S)$ and $\M(T)$.

\question{
    (b) Show that if $\lambda \in \F$ and $T \in \L(V,W)$, then $\M(\lambda T) = \lambda\M(T)$.
}

    Suppose $\M(T) = A$.
    Then for $k = 1,\dots,n$,
\begin{align*}
        (\lambda T)v_k &= \lambda Tv_k \\
                     &= \lambda \sum_{j=1}^m A_{j,k}w_j \\
                     &= \sum_{j=1}^m (\lambda A_{j,k})w_j .
\end{align*}
    Thus $\M(\lambda T)$ is the $m$ by $n$ matrix in which each entry is the corresponding entry of $\M(T)$ multiplied by the scalar $\lambda$.
\end{document}
