\documentclass[a5paper]{article}
\usepackage{amsmath}
\usepackage{amssymb}
\usepackage[top=1cm,right=1cm,bottom=2cm,left=1cm]{geometry}
\setlength\parindent{0pt}
\setlength\parskip{1em}
%
%\usepackage{xcolor}
%\pagecolor[rgb]{0.1,0.1,0.1}
%\color[rgb]{1.0,1.0,1.0}
%
\begin{document}
\newcommand   \C           {\mathbf{C}}
\newcommand   \R           {\mathbf{R}}
\renewcommand \L           {\mathcal{L}}
\newcommand   \F           {\mathbf{F}}
\renewcommand \P           {\mathcal{P}}
\newcommand   \M           {\mathcal{M}}
\newcommand   \op          {\operatorname}


    3.C.14.
    Suppose $m$ and $n$ are positive integers.
    Prove that the function $A \rightarrow A^t$ is a linear map from $\F^{m,n}$ to $\F^{n,m}$.


    Suppose $A \in \F^{m,n}$ and $\lambda \in \F$.
    For each $j \in \{1,\dots,m\}$ and each $k \in \{1,\dots,n\}$,
\begin{align*}
        ((\lambda A)^t)_{k,j} &= (\lambda A)_{j,k} \\
                              &= \lambda A_{j,k} \\
                              &= \lambda (A^t)_{k,j} .
\end{align*}
    Thus the function is homogeneous.

    Now suppose $B, C \in \F^{m,n}$.
    For each $j \in \{1,\dots,m\}$ and each $k \in \{1,\dots,n\}$,
\begin{align*}
        ((B+C)^t)_{k,j} &= (B+C)_{j,k} \\
                        &= B_{j,k} + C_{j,k} \\
                        &= (B^t)_{k,j} + (C^t)_{k,j} .
\end{align*}
    Thus the function is additive.

    Hence the function is a linear map.
\end{document}
